Axiomatize opaque definitions

src/proof/deepcopy.v
@@ -2,6 +2,7 @@ Require Export New.proof.sync.
 From proof.k8s_io.api.apps Require Export v1_init.
 From proof.k8s_io.api.core Require Export v1_init.
 From proof.k8s_io.apimachinery.pkg.apis.meta Require Export v1_init.
+From New.proof Require Export time.
 From proof Require Import prelude empty_ffi.
 
 Section proof.
@@ -10,49 +11,91 @@ Context `{hG: !heapGS Σ} {go_ctx: GoContext}.
 Definition symmetric_iProp {A} (R : A → A → iProp Σ) :=
   ∀ x y, R x y ⊣⊢ R y x.
 
-(* TODO: finish the deepcopy definition *)
-
-Definition deepcopy_of_w32_loc (src dst: loc) : iProp Σ :=
+Definition deepcopy_w32_loc (src dst: loc) : iProp Σ :=
   ⌜src = null ↔ dst = null⌝ ∧
   ∀ (v1 v2: w32), src ↦ v1 -∗ dst ↦ v2 -∗ ⌜ v1 = v2 ⌝.
 
-Definition deepcopy_of_type_meta (src dst: v1.TypeMeta.t) : iProp Σ :=
+Definition deepcopy_w64_loc (src dst: loc) : iProp Σ :=
+  ⌜src = null ↔ dst = null⌝ ∧
+  ∀ (v1 v2: w64), src ↦ v1 -∗ dst ↦ v2 -∗ ⌜ v1 = v2 ⌝.
+
+Definition deepcopy_gmap_string_string (src dst: loc) : iProp Σ :=
+  ⌜src = null ↔ dst = null⌝ ∧
+  ∀ (v1 v2: gmap go_string go_string), src ↦$ v1 -∗ dst ↦$ v2 -∗ ⌜ v1 = v2 ⌝.
+
+Axiom deepcopy_Time: time.Time.t → time.Time.t → iProp Σ.
+
+Definition deepcopy_Time_loc (src dst: loc) : iProp Σ :=
+  ⌜src = null ↔ dst = null⌝ ∧
+  ∀ (v1 v2: time.Time.t), src ↦ v1 -∗ dst ↦ v2 -∗ deepcopy_Time v1 v2.
+
+Axiom deepcopy_OwnerReference: v1.OwnerReference.t → v1.OwnerReference.t → iProp Σ.
+
+Definition deepcopy_list_OwnerReference (src dst: slice.t) : iProp Σ :=
+  ⌜src = slice.nil ↔ dst = slice.nil⌝ ∧
+  ∀ (vs1 vs2: list v1.OwnerReference.t), src ↦* vs1 -∗ dst ↦* vs2 -∗
+    [∗ list] v1;v2 ∈ vs1;vs2, deepcopy_OwnerReference v1 v2.
+
+Definition deepcopy_list_string (src dst: slice.t) : iProp Σ :=
+  ⌜src = slice.nil ↔ dst = slice.nil⌝ ∧
+  ∀ (vs1 vs2: list go_string), src ↦* vs1 -∗ dst ↦* vs2 -∗ ⌜ vs1 = vs2 ⌝.
+
+Axiom deepcopy_ManagedFieldsEntry: v1.ManagedFieldsEntry.t → v1.ManagedFieldsEntry.t → iProp Σ.
+
+Definition deepcopy_list_ManagedFieldsEntry (src dst: slice.t) : iProp Σ :=
+  ⌜src = slice.nil ↔ dst = slice.nil⌝ ∧
+  ∀ (vs1 vs2: list v1.ManagedFieldsEntry.t), src ↦* vs1 -∗ dst ↦* vs2 -∗
+    [∗ list] v1;v2 ∈ vs1;vs2, deepcopy_ManagedFieldsEntry v1 v2.
+
+Definition deepcopy_TypeMeta (src dst: v1.TypeMeta.t) : iProp Σ :=
   ⌜ src = dst ⌝.
 
-Definition deepcopy_of_object_meta (src dst: v1.ObjectMeta.t) : iProp Σ :=
+Definition deepcopy_ObjectMeta (src dst: v1.ObjectMeta.t) : iProp Σ :=
+  ⌜ src.(v1.ObjectMeta.Name') = dst.(v1.ObjectMeta.Name') ∧
+    src.(v1.ObjectMeta.GenerateName') = dst.(v1.ObjectMeta.GenerateName') ∧
+    src.(v1.ObjectMeta.Namespace') = dst.(v1.ObjectMeta.Namespace') ∧
+    src.(v1.ObjectMeta.SelfLink') = dst.(v1.ObjectMeta.SelfLink') ∧ 
+    src.(v1.ObjectMeta.UID') = dst.(v1.ObjectMeta.UID') ∧ 
+    src.(v1.ObjectMeta.ResourceVersion') = dst.(v1.ObjectMeta.ResourceVersion') ∧
+    src.(v1.ObjectMeta.Generation') = dst.(v1.ObjectMeta.Generation') ∧
+    src.(v1.ObjectMeta.CreationTimestamp') = dst.(v1.ObjectMeta.CreationTimestamp') ⌝ ∗
+  deepcopy_Time_loc src.(v1.ObjectMeta.DeletionTimestamp') dst.(v1.ObjectMeta.DeletionTimestamp') ∗
+  deepcopy_w64_loc src.(v1.ObjectMeta.DeletionGracePeriodSeconds') dst.(v1.ObjectMeta.DeletionGracePeriodSeconds') ∗
+  deepcopy_gmap_string_string src.(v1.ObjectMeta.Labels') dst.(v1.ObjectMeta.Labels') ∗
+  deepcopy_gmap_string_string src.(v1.ObjectMeta.Annotations') dst.(v1.ObjectMeta.Annotations') ∗
+  deepcopy_list_OwnerReference src.(v1.ObjectMeta.OwnerReferences') dst.(v1.ObjectMeta.OwnerReferences') ∗
+  deepcopy_list_string src.(v1.ObjectMeta.Finalizers') dst.(v1.ObjectMeta.Finalizers') ∗
+  deepcopy_list_ManagedFieldsEntry src.(v1.ObjectMeta.ManagedFields') dst.(v1.ObjectMeta.ManagedFields').
+
+Axiom deepcopy_PodSpec: v1.PodSpec.t → v1.PodSpec.t → iProp Σ.
+
+Axiom deepcopy_PodStatus: v1.PodStatus.t → v1.PodStatus.t → iProp Σ.
+
+Definition deepcopy_Pod (src dst: v1.Pod.t) : iProp Σ :=
+  deepcopy_TypeMeta src.(v1.Pod.TypeMeta') dst.(v1.Pod.TypeMeta') ∗
+  deepcopy_ObjectMeta src.(v1.Pod.ObjectMeta') dst.(v1.Pod.ObjectMeta') ∗
+  deepcopy_PodSpec src.(v1.Pod.Spec') dst.(v1.Pod.Spec') ∗
+  deepcopy_PodStatus src.(v1.Pod.Status') dst.(v1.Pod.Status').
+
+Definition deepcopy_ReplicaSetSpec (src dst: v1.ReplicaSetSpec.t) : iProp Σ :=
+  deepcopy_w32_loc src.(v1.ReplicaSetSpec.Replicas') dst.(v1.ReplicaSetSpec.Replicas').
+
+Definition deepcopy_ReplicaSetStatus (src dst: v1.ReplicaSetStatus.t) : iProp Σ :=
   True%I.
 
-Definition deepcopy_of_pod_spec (src dst: v1.PodSpec.t) : iProp Σ :=
-  True%I.
+Definition deepcopy_ReplicaSet (src dst: v1.ReplicaSet.t) : iProp Σ :=
+  deepcopy_TypeMeta src.(v1.ReplicaSet.TypeMeta') dst.(v1.ReplicaSet.TypeMeta') ∗
+  deepcopy_ObjectMeta src.(v1.ReplicaSet.ObjectMeta') dst.(v1.ReplicaSet.ObjectMeta') ∗
+  deepcopy_ReplicaSetSpec src.(v1.ReplicaSet.Spec') dst.(v1.ReplicaSet.Spec') ∗
+  deepcopy_ReplicaSetStatus src.(v1.ReplicaSet.Status') dst.(v1.ReplicaSet.Status').
 
-Definition deepcopy_of_pod_status (src dst: v1.PodStatus.t) : iProp Σ :=
-  True%I.
-
-Definition deepcopy_of_pod (src dst: v1.Pod.t) : iProp Σ :=
-  deepcopy_of_type_meta src.(v1.Pod.TypeMeta') dst.(v1.Pod.TypeMeta') ∗
-  deepcopy_of_object_meta src.(v1.Pod.ObjectMeta') dst.(v1.Pod.ObjectMeta') ∗
-  deepcopy_of_pod_spec src.(v1.Pod.Spec') dst.(v1.Pod.Spec') ∗
-  deepcopy_of_pod_status src.(v1.Pod.Status') dst.(v1.Pod.Status').
-
-Definition deepcopy_of_replicaset_spec (src dst: v1.ReplicaSetSpec.t) : iProp Σ :=
-  deepcopy_of_w32_loc src.(v1.ReplicaSetSpec.Replicas') dst.(v1.ReplicaSetSpec.Replicas').
-
-Definition deepcopy_of_replicaset_status (src dst: v1.ReplicaSetStatus.t) : iProp Σ :=
-  True%I.
-
-Definition deepcopy_of_replicaset (src dst: v1.ReplicaSet.t) : iProp Σ :=
-  deepcopy_of_type_meta src.(v1.ReplicaSet.TypeMeta') dst.(v1.ReplicaSet.TypeMeta') ∗
-  deepcopy_of_object_meta src.(v1.ReplicaSet.ObjectMeta') dst.(v1.ReplicaSet.ObjectMeta') ∗
-  deepcopy_of_replicaset_spec src.(v1.ReplicaSet.Spec') dst.(v1.ReplicaSet.Spec') ∗
-  deepcopy_of_replicaset_status src.(v1.ReplicaSet.Status') dst.(v1.ReplicaSet.Status').
-
-Lemma deepcopy_of_pod_symmetric:
-  symmetric_iProp deepcopy_of_pod.
+Lemma deepcopy_Pod_symmetric:
+  symmetric_iProp deepcopy_Pod.
 Proof.
 Admitted.
 
-Lemma deepcopy_of_replicaset_symmetric:
-  symmetric_iProp deepcopy_of_replicaset.
+Lemma deepcopy_ReplicaSet_symmetric:
+  symmetric_iProp deepcopy_ReplicaSet.
 Proof.
 Admitted.
 
